updates

intermediate/Veritas.Intermediate.Store.fst
@@ -134,6 +134,11 @@ let bevict_from_store
 
 let store_contains_key (#vcfg:_) (st:vstore vcfg) (k:key): bool  = admit()
 
+let lemma_stored_key_implies_contains (#vcfg:_) (st: vstore vcfg) (s:inuse_slot_id st):
+  Lemma (ensures (store_contains_key st (stored_key st s)))
+  = admit()
+
+
 let slot_of_key (#vcfg:_) (st:vstore vcfg) (k:key{store_contains_key st k}): 
   (s:inuse_slot_id st{stored_key st s = k}) = admit()
 
@@ -169,6 +174,13 @@ let lemma_as_map_slot_key_equiv (#vcfg:_) (st:ismap_vstore vcfg) (s:slot_id vcfg
                     stored_value st s = Spec.stored_value (as_map st) k /\
                     add_method_of st s = Spec.add_method_of (as_map st) k))
   = admit()
+
+let lemma_as_map_slot_key_equiv2 (#vcfg:_) (st:ismap_vstore vcfg) (s:inuse_slot_id _)
+  : Lemma (ensures (let k = stored_key st s in
+                    let stk = as_map st in
+                    Spec.store_contains stk k /\
+                    stored_value st s = Spec.stored_value stk k /\
+                    add_method_of st s = Spec.add_method_of stk k)) = admit()
 
 
 let lemma_store_rel_contains_key (#vcfg:_) (st:vstore vcfg) (st':Spec.vstore) (k:key)
